fixtures/TypeChecker.mli
@@ -817,8 +817,8 @@ val wf_outlives_b : region_ctx -> outlives_ctx -> bool
 val outlives_constraints_hold_b : outlives_ctx -> outlives_ctx -> bool
 
 val infer_hrt_call_env :
-  outlives_ctx -> Big_int_Z.big_int -> outlives_ctx -> ty -> ty list -> ty
-  infer_result
+  outlives_ctx -> Big_int_Z.big_int -> Big_int_Z.big_int -> outlives_ctx ->
+  ty -> ty list -> ty infer_result
 
 val open_core_trait_bounds :
   lifetime option list -> ty core_trait_bound list -> ty core_trait_bound list
