rocq/theories/TypeSystem/AlphaRoots.v
@@ -317,6 +317,20 @@ Inductive typed_env_roots_shadow_safe
         (params_of_tys (map (open_bound_ty σ) param_tys)) Σ' R' arg_roots ->
       typed_env_roots_shadow_safe env Ω n R Σ (ECallExpr callee args)
         (open_bound_ty σ ret) Σ' R' (root_set_union roots_callee (root_sets_union arg_roots))
+  | TERS_CallExpr_Forall_Closure : forall R R1 R' Σ Σ1 Σ' callee args u
+      m bounds body_ty env_lt param_tys ret σ arg_roots roots_callee,
+      (forall fname caps, callee <> EMakeClosure fname caps) ->
+      typed_env_roots_shadow_safe env Ω n R Σ callee
+        (MkTy u (TForall m bounds body_ty)) Σ1 R1 roots_callee ->
+      ty_core body_ty = TClosure env_lt param_tys ret ->
+      contains_lbound_lifetime (open_bound_lifetime σ env_lt) = false ->
+      contains_lbound_ty (open_bound_ty σ ret) = false ->
+      contains_lbound_outlives (open_bound_outlives σ bounds) = false ->
+      Forall (fun '(a, b) => outlives Ω a b) (open_bound_outlives σ bounds) ->
+      typed_args_roots_shadow_safe env Ω n R1 Σ1 args
+        (params_of_tys (map (open_bound_ty σ) param_tys)) Σ' R' arg_roots ->
+      typed_env_roots_shadow_safe env Ω n R Σ (ECallExpr callee args)
+        (open_bound_ty σ ret) Σ' R' (root_set_union roots_callee (root_sets_union arg_roots))
   | TERS_Struct : forall R R' Σ Σ' sname lts args fields sdef roots,
       Program.lookup_struct sname env = Some sdef ->
       Datatypes.length lts = Program.struct_lifetimes sdef ->
@@ -1070,6 +1084,32 @@ Proof.
     exists R20, (root_set_union roots_callee0 (root_sets_union arg_roots0)).
     split; [| split; [| split]].
     + eapply TERS_CallExpr_Forall_Fn; eauto.
+    + exact HnsR20.
+    + exact HR20.
+    + eapply root_set_equiv_trans.
+      * apply root_set_union_equiv.
+       -- exact Hroots_callee0.
+       -- eapply root_set_equiv_trans.
+          ++ apply root_sets_union_equiv. exact Harg_roots0.
+          ++ apply root_set_equiv_sym. apply root_sets_instantiate_union_equiv.
+      * apply root_set_equiv_sym. apply root_set_instantiate_union_equiv.
+  - intros R R1 R' Σ Σ1 Σ' callee args u m bounds body_ty env_lt
+      param_tys ret σ arg_roots roots_callee Hnot_mc Hcallee IHcallee Hbody
+      Henv_ok Hret_ok Hbounds_ok Hout Hargs IHargs Hfresh R0 HnsR HnsR0 HR0.
+    rewrite expr_local_store_names_call_expr in Hfresh.
+    apply root_subst_images_exclude_names_app_inv in Hfresh.
+    destruct Hfresh as [Hfresh_callee Hfresh_args].
+    destruct (IHcallee Hfresh_callee R0 HnsR HnsR0 HR0)
+      as [R10 [roots_callee0 [Hcallee0 [HnsR10 [HR10 Hroots_callee0]]]]].
+    assert (Hns_R1 : root_env_no_shadow R1).
+    { eapply typed_env_roots_no_shadow.
+      - eapply typed_env_roots_shadow_safe_roots. exact Hcallee.
+      - exact HnsR. }
+    destruct (IHargs Hfresh_args R10 Hns_R1 HnsR10 HR10)
+      as [R20 [arg_roots0 [Hargs0 [HnsR20 [HR20 Harg_roots0]]]]].
+    exists R20, (root_set_union roots_callee0 (root_sets_union arg_roots0)).
+    split; [| split; [| split]].
+    + eapply TERS_CallExpr_Forall_Closure; eauto.
     + exact HnsR20.
     + exact HR20.
     + eapply root_set_equiv_trans.
